Foundation/Modal/Kripke/AxiomWeakDot2.lean
@@ -1,0 +1,58 @@
+import Foundation.Modal.Kripke.Completeness
+
+namespace LO.Modal
+
+namespace Kripke
+
+
+section definability
+
+open Formula.Kripke
+
+variable {F : Kripke.Frame}
+
+lemma weakConnected_of_validate_WeakDot2 (hCon : WeakConfluent F) : F ⊧ (Axioms.WeakDot2 (.atom 0) (.atom 1)) := by sorry
+
+lemma validate_WeakDot2_of_weakConfluent : F ⊧ (Axioms.WeakDot2 (.atom 0) (.atom 1)) → WeakConfluent F := by sorry;
+
+abbrev WeakConfluentFrameClass : FrameClass := { F | WeakConfluent F }
+
+instance : WeakConfluentFrameClass.IsNonempty := by
+  use ⟨Unit, λ _ _ => True⟩;
+  simp [WeakConfluent];
+
+instance WeakConfluentFrameClass.DefinedByWeakDot2 : WeakConfluentFrameClass.DefinedBy {Axioms.WeakDot2 (.atom 0) (.atom 1)} := ⟨by
+  intro F;
+  constructor;
+  . simpa using weakConnected_of_validate_WeakDot2;
+  . simpa using validate_WeakDot2_of_weakConfluent;
+⟩
+
+end definability
+
+
+section canonicality
+
+variable {S} [Entailment (Formula ℕ) S]
+variable {𝓢 : S} [Entailment.Consistent 𝓢] [Entailment.K 𝓢]
+
+open Formula.Kripke
+open Entailment
+open MaximalConsistentTableau
+open canonicalModel
+
+namespace Canonical
+
+lemma weakConfluent [Entailment.HasAxiomWeakDot2 𝓢] : WeakConfluent (canonicalFrame 𝓢).Rel := by
+  rintro x y z ⟨Rxy, Rxz, eyz⟩;
+  by_contra hC;
+  sorry;
+
+end Canonical
+
+end canonicality
+
+
+end Kripke
+
+end LO.Modal
