Foundation/Modal/Tableau.lean
@@ -375,8 +375,17 @@ lemma equality_of₁ (e₁ : t₁.1.1 = t₂.1.1) : t₁ = t₂ := by
 
 lemma equality_of₂ (e₂ : t₁.1.2 = t₂.1.2) : t₁ = t₂ := equality_of₁ $ maximal_duality.mpr e₂
 
+lemma ne₁_of_ne : t₁ ≠ t₂ → t₁.1.1 ≠ t₂.1.1 := by
+  contrapose;
+  push_neg;
+  exact equality_of₁;
 
-lemma intro_equality {h₁ : ∀ {φ}, φ ∈ t₁.1.1 → φ ∈ t₂.1.1} {h₂ : ∀ {φ}, φ ∈ t₁.1.2 → φ ∈ t₂.1.2} : t₁ = t₂ := by
+lemma ne₂_of_ne : t₁ ≠ t₂ → t₁.1.2 ≠ t₂.1.2 := by
+  contrapose;
+  push_neg;
+  exact equality_of₂;
+
+lemma intro_equality (h₁ : ∀ {φ}, φ ∈ t₁.1.1 → φ ∈ t₂.1.1) (h₂ : ∀ {φ}, φ ∈ t₁.1.2 → φ ∈ t₂.1.2) : t₁ = t₂ := by
   apply equality_of₁;
   apply Set.eq_of_subset_of_subset;
   . intro φ hφ;
